To check if a **subarray with sum = 0** exists, the logic revolves around prefix sums and their properties. Here's how this can be efficiently determined:

---

### Observations:

1. **Subarray Sum Property:**
    
    - The sum of a subarray sum(i,j)=0\text{sum}(i, j) = 0 implies: PS[j]=PS[i−1]\text{PS}[j] = \text{PS}[i-1] This means that if two prefix sums are equal, the subarray between those indices has a sum of 0.
2. **Prefix Sum Array:**
    
    - Compute the prefix sum PS[i]=arr[0]+arr[1]+⋯+arr[i]\text{PS}[i] = \text{arr}[0] + \text{arr}[1] + \dots + \text{arr}[i].
    - If the prefix sum at any index becomes zero, it means the subarray from the beginning of the array to that index has a sum of 0.
3. **Using a HashMap for Optimization:**
    
    - A hashmap (dictionary) is used to store the prefix sums.
    - If a prefix sum repeats, it indicates the presence of a subarray with sum = 0.
    - The hashmap allows for O(1)O(1) lookup time, making the solution efficient.

---

### Steps:

1. **Initialize a HashMap:**
    
    - Use the hashmap to store prefix sums and their first occurrence index (optional if we don't need to print the subarray).
2. **Traverse the Array:**
    
    - Maintain a running prefix sum.
    - If the prefix sum is 0 or already exists in the hashmap, return `True`.
    - Otherwise, add the prefix sum to the hashmap.
3. **Handle Edge Cases:**
    
    - If the array contains 0, directly return `True` as a single-element subarray can have sum 0.

---

### Algorithm:

1. Check if 0 exists in the array. If yes, return `True`.
2. Initialize a prefix sum variable as 0.
3. Traverse the array and update the prefix sum.
4. Check if the prefix sum is already in the hashmap or equals 0. If yes, return `True`.
5. Otherwise, add the prefix sum to the hashmap.
6. If no such subarray is found, return `False`.

---

### Code (Python):

```python
def has_zero_sum_subarray(arr):
    prefix_sum = 0
    seen_sums = set()

    for num in arr:
        prefix_sum += num

        # Check if prefix_sum is 0 or already exists
        if prefix_sum == 0 or prefix_sum in seen_sums:
            return True
        
        # Add prefix_sum to the set
        seen_sums.add(prefix_sum)

    return False


# Example
arr = [3, 4, -7, 1, 3, 3, 1, -4]
print(has_zero_sum_subarray(arr))  # Output: True
```

---

### Example Walkthrough:

#### Input:

`arr = [3, 4, -7, 1, 3, 3, 1, -4]`

#### Steps:

1. **Initial State:**
    
    - `prefix_sum = 0`
    - `seen_sums = {}`
2. **Iteration 1:**
    
    - `num = 3, prefix_sum = 3`
    - Add `3` to `seen_sums`: `{3}`.
3. **Iteration 2:**
    
    - `num = 4, prefix_sum = 7`
    - Add `7` to `seen_sums`: `{3, 7}`.
4. **Iteration 3:**
    
    - `num = -7, prefix_sum = 0`
    - Prefix sum is `0`, so return `True`.

---

### Complexity:

1. **Time Complexity:**
    
    - O(N)O(N), where NN is the size of the array.
    - Each element is processed once, and hashmap lookups/insertions take O(1)O(1).
2. **Space Complexity:**
    
    - O(N)O(N) for the hashmap storing prefix sums.

---

### Extensions:

- To **print the subarray**, store the first occurrence index of each prefix sum in the hashmap. When a duplicate is found, the subarray is from the next index of the first occurrence to the current index.

**Modified Code to Print Subarray:**

```python
def find_zero_sum_subarray(arr):
    prefix_sum = 0
    sum_index_map = {}

    for i, num in enumerate(arr):
        prefix_sum += num

        if prefix_sum == 0:
            return arr[:i + 1]

        if prefix_sum in sum_index_map:
            return arr[sum_index_map[prefix_sum] + 1 : i + 1]
        
        sum_index_map[prefix_sum] = i

    return None


# Example
arr = [3, 4, -7, 1, 3, 3, 1, -4]
print(find_zero_sum_subarray(arr))  # Output: [3, 4, -7]
```

This approach efficiently handles the problem and provides flexibility to return just the boolean result or the actual subarray.